ghost state machine example progress

pulse/share/steel/examples/pulse/GhostState.fst
@@ -6,25 +6,40 @@ open Pulse.Lib.SpinLock
 assume
 val run_stt (#a:Type) (#post:a -> vprop) (f:stt a emp post) : a
 
-type st_t =
+type pure_st_t =
   | Init
   | Next
   | Final
 
-// assume
-// val payload_t : Type0
+assume
+val payload_t : Type0
 
-// noeq
-// type concrete_st_t = 
-//   | CInit 
-//   | CNext : payload_t -> concrete_st_t
-//   | CState2 : payload_t -> concrete_st_t
+noeq
+type st_t = 
+  | CInit
+  | CNext : payload_t -> st_t
+  | CFinal : payload_t -> st_t
+
+type pure_handle_t = ref pure_st_t
 
 type handle_t = ref st_t
 
-let handle_has_state (h:handle_t) (s:st_t) : vprop = pts_to h #half_perm s
+let pure_handle_has_state (h:pure_handle_t) (s:pure_st_t) : vprop = pts_to h #half_perm s
 
-type locked_handle_t = h:handle_t & lock (exists_ (fun s -> handle_has_state h s))
+let handle_has_state (h:handle_t) (s:st_t) : vprop = pts_to h s
+
+let states_correspond (s:st_t) (ps:pure_st_t) : prop
+  = (CInit? s) /\ (Init? ps)
+  \/(CNext? s) /\ (Next? ps)
+  \/(CFinal? s) /\ (Final? ps)
+
+type locked_state_t = h:handle_t 
+                    & ph:pure_handle_t 
+                    & lock (exists_ (fun s ->
+                            exists_ (fun ps -> 
+                                handle_has_state h s **
+                                pure_handle_has_state ph ps **
+                                pure (states_correspond s ps))))
 
 // -------------------------------------------------------------------------- //
 
@@ -32,57 +47,75 @@ type locked_handle_t = h:handle_t & lock (exists_ (fun s -> handle_has_state h s
 ```pulse
 fn init' (_:unit)
   requires emp
-  returns p:locked_handle_t
-  ensures handle_has_state p._1 Init
+  returns tup:locked_state_t
+  ensures pure_handle_has_state tup._2 Init
 {
-  let h = alloc Init;
-  share #st_t #emp_inames h #Init;
-  fold handle_has_state h Init;
-  fold handle_has_state h Init;
-  let lk = new_lock (exists_ (fun s -> handle_has_state h s));
-  let p = (| h, lk |);
-  rewrite (handle_has_state h Init)
-       as (handle_has_state p._1 Init);
+  let ph = alloc Init;
+  let h = alloc CInit;
+
+  share #pure_st_t #emp_inames ph #Init;
+  fold pure_handle_has_state ph Init;
+  fold pure_handle_has_state ph Init;
+  fold handle_has_state h CInit;
+
+  let lk = new_lock (exists_ (fun s ->
+                     exists_ (fun ps -> 
+                        handle_has_state h s **
+                        pure_handle_has_state ph ps **
+                        pure (states_correspond s ps))));
+
+  let tup = (| h, ph, lk |);
+  rewrite (pure_handle_has_state ph Init)
+       as (pure_handle_has_state tup._2 Init);
 
   // FIXME: cannot prove 
-  //   handle_has_state (Mkdtuple2?._1 x) Init 
+  //   pure_handle_has_state (Mkdtuple3?._2 x) Init 
   // in the context
-  //   handle_has_state (Mkdtuple2?._1 p) Init
+  //   pure_handle_has_state (Mkdtuple3?._2 p) Init
   // ISSUE: idk
-  
-  p
+
+  ph
 }
 ```
-let global_locked_handle : locked_handle_t = admit() // run_stt (init' ())
+let global_locked_state : locked_state_t = admit() // run_stt (init' ())
 
 #set-options "--print_implicits"
+
+assume
+val some_payload : payload_t
 
 [@@expect_failure]
 ```pulse
 fn next' (_:unit)
-  requires handle_has_state global_locked_handle._1 Init
-  ensures handle_has_state global_locked_handle._1 Next
+  requires pure_handle_has_state global_locked_state._2 Init
+  ensures pure_handle_has_state global_locked_state._2 Next
 {
-  acquire global_locked_handle._2;
-  with s. assert (handle_has_state global_locked_handle._1 s);
-  unfold handle_has_state global_locked_handle._1 Init;
-  unfold handle_has_state global_locked_handle._1 s;
+  acquire global_locked_state._3;
+  with s. assert (handle_has_state global_locked_state._1 s);
+  with ps. assert (pure_handle_has_state global_locked_state._2 ps);
+  unfold handle_has_state global_locked_state._1 s;
+  unfold pure_handle_has_state global_locked_state._2 Init;
+  unfold pure_handle_has_state global_locked_state._2 ps;
 
-  // FIXME: cannot prove
-  //   pts_to #st_t (Mkdtuple2?._1 #handle_t #(fun h -> lock (exists_ #st_t (fun s -> handle_has_state h s))) global_locked_handle) #half_perm Init
-  // in the context
-  //   pts_to #st_t (Mkdtuple2?._1 #handle_t #(fun h -> lock (exists_ #st_t (fun s -> pts_to #st_t h #half_perm s <: Prims.Tot vprop))) global_locked_handle) #half_perm Init
   // ISSUE: the unfold of
-  //   handle_has_state global_locked_handle._1 s
+  //   pure_handle_has_state global_locked_state._2 ps
   // unfolded too much, so now there is not syntactic equality 
 
-  pts_to_injective_eq #st_t #half_perm #half_perm #Init #s global_locked_handle._1;
-  rewrite (pts_to global_locked_handle._1 #half_perm s)
-       as (pts_to global_locked_handle._1 #half_perm Init);
-  gather #st_t #emp_inames global_locked_handle._1 #Init;
-  global_locked_handle._1 := Next;
-  share #st_t #emp_inames global_locked_handle._1 #Next;
-  fold handle_has_state global_locked_handle._1 Next;
-  release global_locked_handle._2;
+  pts_to_injective_eq #pure_st_t #half_perm #half_perm #Init #ps global_locked_state._2;
+  rewrite (pts_to global_locked_state._2 #half_perm ps)
+       as (pts_to global_locked_state._2 #half_perm Init);
+  gather #pure_st_t #emp_inames global_locked_state._2 #Init;
+
+  let st = CNext some_payload;
+  global_locked_state._1 := st;
+  global_locked_state._2 := Next;
+
+  share #pure_st_t #emp_inames global_locked_state._2 #Next;
+  fold pure_handle_has_state global_locked_state._2 Next;
+  fold pure_handle_has_state global_locked_state._2 Next;
+  fold handle_has_state global_locked_state._2 st;
+  assert (pure (states_correspond st Next));
+
+  release global_locked_state._3;
 }
 ```
